proved that evaln commutes with L4 to L4_1, using parametricity.
the proof that the L4 and L4_1 instantiations of the TermAbs
interface are parametrically related has some admits and needs
discussion with Matthieu.

L4 uses a concrete de-bruijn representation (L4.expression.exp).
L4_1 uses an abstract (SquiggleEq style) de-bruijn representation.

Also, removed the remaining admit in the L4_2 to L4_5 proof in
r7892.

(branch L4param)

theories/L4_deBruijn/L4_to_L4_2_correct.v
@@ -22,12 +22,47 @@ Require Import SquiggleEq.tactics.
 Require Import Coq.Unicode.Utf8.
 Require Import List.
 Require Import SquiggleEq.list.
+(* Move to SquiggleEq.list *)
+Hint Rewrite app_length repeat_length firstn_length : list.
+(* Move to SquiggleEq.list *)
+Lemma listPadId {A:Type} d (l: list A) n :
+  (n <= length l)%nat -> listPad d l n = l.
+Proof using.
+  clear.
+  intros Hyp.
+  unfold listPad.
+  assert (n-length l =0)%nat  as Heq by omega.
+  rewrite Heq. simpl.
+  autorewrite with list. refl.
+Qed.
+
 
 Open Scope program_scope.
 
 
 Open Scope N_scope.
+Require Import Common.TermAbs_parametricity.
 
+Parametricity Recursive eval_n.
+Require Import L4.variables.
+
+
+(* should be automatically provalble for all types with decidable equality.
+  However, it cannot be internally stated. *)
+Global Instance EqIfRdcon : EqIfR L4_o_polyEval_o_dcon_R.
+Proof using.
+Admitted.
+
+Global Instance EqIfRstring : EqIfR string_R.
+Proof using.
+Admitted.
+
+Global Instance EqIfRL4Opid : EqIfR L4Opid_R.
+Proof using.
+  constructor; intros Hyp; subst.
+- inverts Hyp; auto; f_equal; try apply eqIfR; auto.
+  unfold dcon in *.
+Admitted.
 Section L4Inst.
 
 
@@ -40,9 +75,11 @@ and return None if they are not met.
 Although the former choice avoids checks, it may end up paying large performance
 penalties for carrying around proofs. Also, carrying around proofs make 
 it hard to write down programs without using tactics.
-In the latter choice, if the checks are indeed too costly,
+In the latter choice, if the checks are indeed too costly (note that these
+checks are only in the evaln function, which is only for debugging purposes),
 we can later prove that on closed inputs, the eval function
 produces the same answer as another one that doesn't do the checks.
+
 
 Some day, there should be an unconditional proof of substitution commuting with
 DB to named conversion.
@@ -78,8 +115,9 @@ match t  return option (L4Opid * list BTerm) with
     let ns := map fst fs in
     Some (NFix (length fs) (N.to_nat n), map (fun e => (ns,snd e)) fs)
 
-(** Fix : An axiom behaves differently from a constructor: (Ax _) --> Ax *)
-| Ax_e s => Some (NDCon (dummyind,0) 0, [])
+| Ax_e s => Some (NBox s, [])
+(** based on  L4_to_L4_1_to_L4_2 tL4_to_L4_1*)
+| Prf_e => Some (NBox "proof", [])
 end.
 
 Require Import ExtLib.Structures.Monads.
@@ -126,7 +164,7 @@ else
 
 Require Import TermAbs.
 Definition L4Abs : Common.TermAbs.TermAbs L4Opid :=
-(@Build_TermAbs _ _ 
+(@Build_TermAbs _
   Term 
   BTerm 
   numBvars 
@@ -136,25 +174,100 @@ Definition L4Abs : Common.TermAbs.TermAbs L4Opid :=
   fromOpidBTerms
   (fun e => ([],e))).
 
-End L4Inst.
 
-Require Import Common.TermAbs_parametricity.
+Require Import SquiggleEq.termsDB.
+Definition bL4_to_L4_1 (b:BTerm) : @DBTerm Ast.name L4Opid :=
+  termsDB.bterm (fst b) (tL4_to_L4_1 (snd b)).
 
-Parametricity Recursive eval_n.
 Require Import L4.variables.
 
-(* should be automatically provalble for all types with decidable equality.
-  However, it cannot be internally stated. *)
-Global Instance EqIfRL4Opid : EqIfR L4Opid_R.
-Proof using.
-  constructor; intros Hyp; subst.
-- inverts Hyp; auto; f_equal; try apply eqIfR; auto.
-  unfold dcon in *.
+Lemma L4L41toOpidBtermsR:
+   ∀ (H : exp) (H0 : DTerm),
+  tL4_to_L4_1 H = H0
+  → option_R (L4Opid * list BTerm) (L4Opid * list DBTerm)
+      (prod_R L4Opid L4Opid L4Opid_R (list BTerm) (list DBTerm)
+         (list_R BTerm DBTerm (λ (b4 : BTerm) (b41 : DBTerm), bL4_to_L4_1 b4 = b41)))
+      (toOpidBTerms H) (getOpidBTerms H0).
+Proof.
+- intros d ? Hal. subst. 
+  destruct d; simpl; repeat constructor; try apply eqIfR; try refl.
+  + clear. induction e; auto; simpl; congruence.
+  + clear. induction e; constructor; eauto.
+  + clear. induction b; auto; simpl in *. destruct p. simpl; f_equal; eauto.
+    f_equal. unfold num_bvars. simpl.
+    unfold listPad. autorewrite with list. lia.
+  + clear.  simpl.  induction b; simpl; try constructor; eauto.
+    destruct p; constructor; eauto.
+  (* need to remove the listPad business. it comes from tL4_to_L4_1 
+In brcons_e, there is a number used for db computations as # bound vars.
+Then there are names. would the names have the same length as n.
+If not, using listPad. update getOpidBterms to also do the padding
+   *)
 Admitted.
 
+Lemma L4L41applyBTerm:
+ ∀ (H : BTerm) (H0 : DBTerm),
+  bL4_to_L4_1 H = H0
+  → ∀ (H1 : list exp) (H2 : list DTerm),
+    list_R exp DTerm (λ (t4 : exp) (t41 : DTerm), tL4_to_L4_1 t4 = t41) H1 H2
+    → option_R exp DTerm (λ (t4 : exp) (t41 : DTerm), tL4_to_L4_1 t4 = t41) 
+               (applyBTerm H H1) (applyBTermClosed Ast.name L4Opid H0 H2).
+Proof.
+Admitted.
+
+Lemma L4L41fromOpidBtermsR:
+  ∀ (H : list BTerm) (H0 : list DBTerm),
+  list_R BTerm DBTerm (λ (b4 : BTerm) (b41 : DBTerm), bL4_to_L4_1 b4 = b41) H H0
+  → ∀ H1 H2 : L4Opid,
+    L4Opid_R H1 H2
+    → option_R exp DTerm (λ (t4 : exp) (t41 : DTerm), tL4_to_L4_1 t4 = t41) 
+               (fromOpidBTerms H H1) (mkBTermSafe Ast.name L4Opid H0 H2).
+Proof.
+  intros lbt ? Hp ? o Ho. apply eqIfR in Ho. subst.
+  apply list_RP_same in Hp.
+  eapply list_Rext in Hp;
+    [ | intros ? ?;rewrite <- (and_true_l (bL4_to_L4_1 a1 = a2)); tauto].
+  apply list_RP_same in Hp.
+  apply list_R_map in Hp.
+  apply list_R_eq in Hp;[ |  eauto with typeclass_instances]. subst.
+Admitted.
+
+Definition TermAbs_R_L4_L4_1 : 
+  TermAbs_R L4Opid L4Opid L4Opid_R
+    L4Abs    
+    (TermAbsDB Ast.name L4Opid).
+Proof using.
+  eapply TermAbs_R_Build_TermAbs_R with 
+    (AbsTerm_R := fun t4 t41 => tL4_to_L4_1 t4 = t41)
+    (AbsBTerm_R := fun b4 b41 => bL4_to_L4_1 b4 = b41).
+- intros b ? ?. subst.  apply nat_R_eq. destruct b. refl.
+- apply L4L41toOpidBtermsR. 
+- intros t ? Hp. subst; destruct t. simpl. destruct l; simpl; try constructor; refl.
+- apply L4L41applyBTerm.
+- apply L4L41fromOpidBtermsR.
+- intros t ? Hp. subst. refl.
+Defined. (* NOT Qed. the parametricity relations between Terms and BTerms is a part of the proof *)
+
+End L4Inst.
+
+
+Lemma L4_to_L4_1_free_thm:
+  forall (t1 : L4.expression.exp) n,
+    (option_map tL4_to_L4_1 (@eval_n L4Abs n t1))
+    =
+   (@eval_n  (TermAbsDB Ast.name L4Opid) n (tL4_to_L4_1 t1)).
+Proof using.
+  intros ? ?.
+  pose proof (L4_o_polyEval_o_eval_n_R 
+   L4Abs  (TermAbsDB Ast.name L4Opid)
+   TermAbs_R_L4_L4_1 n n ltac:(apply eqIfR; refl) t1 _ eq_refl) as Hp.
+  simpl in Hp.
+  inverts Hp; simpl in *; congruence.
+Qed.  
+  
 Let TermAbs_R_NamedDB2 :=
   (@TermAbs_R_NamedDB Ast.name NVar _ L4Opid _ _ _ _  _ _ Ast.nAnon mkNVar getNId getIdMkNVar
-     L4Opid_R L4_o_polyEval_o_CoqL4GenericTermSig_R EqIfRL4Opid).
+     L4Opid_R EqIfRL4Opid).
 
 Lemma L4_1_to_L4_2_free_thm:
   forall (t1 : L4_1_Term) n,
@@ -177,4 +290,3 @@ Proof using.
   - invertsna Hp Hp. setoid_rewrite <- Hp.
     constructor.
 Qed.
-  
